theories/machine_run.v
@@ -1,0 +1,75 @@
+From stdpp Require Import base.
+From iris.program_logic Require Import language.
+From cap_machine Require Import machine_parameters machine_base cap_lang.
+
+(* The operational semantics as an interpreter: this effectively "runs" the
+   machine until it fails or halts (or we run out of fuel). *)
+
+Fixpoint machine_run `{MachineParameters} (fuel: nat) (c: Conf): option ConfFlag :=
+  match fuel with
+  | 0 => None
+  | S fuel =>
+    match c with
+    | (Failed, _) => Some Failed
+    | (Halted, _) => Some Halted
+    | (NextI, φ) => machine_run fuel (Executable, φ)
+    | (Executable, (r, m)) =>
+      let pc := r !r! PC in
+      if isCorrectPCb pc then (
+        let a := match pc with
+                 | inl _ => top (* dummy *)
+                 | inr (_, _, _, _, a) => a
+                 end in
+        let i := decodeInstrW (m !m! a) in
+        let c' := exec i (r, m) in
+        machine_run fuel (c'.1, c'.2)
+      ) else (
+        Some Failed
+      )
+    end
+  end.
+
+Lemma machine_run_correct `{MachineParameters} fuel cf (φ: ExecConf) cf':
+  machine_run fuel (cf, φ) = Some cf' →
+  ∃ φ', rtc erased_step
+            ([Seq (Instr cf)], φ)
+            ([Instr cf'], φ').
+Proof.
+  revert cf cf' φ. induction fuel.
+  { cbn. done. }
+  { cbn. intros ? ? [r m] Hc.
+    destruct cf; simplify_eq.
+    destruct (isCorrectPCb (r !r! PC)) eqn:HPC.
+    { apply isCorrectPCb_isCorrectPC in HPC.
+      destruct (r !r! PC) as [|c] eqn:Hr; [by inversion HPC|].
+      destruct_cap c.
+      eapply IHfuel in Hc as [φ' Hc]. eexists.
+      eapply rtc_l. unfold erased_step. exists [].
+      eapply step_atomic with (t1:=[]). 1,2: reflexivity. cbn.
+      eapply ectx_language.Ectx_step with (K:=[SeqCtx]). 1,2: reflexivity.
+      constructor. eapply step_exec_instr; eauto. rewrite Hr //.
+      apply Hc. }
+    { simplify_eq. apply isCorrectPCb_nisCorrectPC in HPC.
+      eexists. eapply rtc_l. unfold erased_step. exists [].
+      eapply step_atomic with (t1:=[]). 1,2: reflexivity. cbn.
+      eapply ectx_language.Ectx_step with (K:=[SeqCtx]). 1,2: reflexivity. cbn.
+      constructor. eapply step_exec_fail; eauto.
+      eapply rtc_once. exists [].
+      eapply step_atomic with (t1:=[]). 1,2: reflexivity. cbn.
+      eapply ectx_language.Ectx_step with (K:=[]). 1,2: reflexivity. cbn.
+      constructor. }
+    { eexists. eapply rtc_once. exists [].
+      eapply step_atomic with (t1:=[]). 1,2: reflexivity. cbn.
+      eapply ectx_language.Ectx_step with (K:=[]). 1,2: reflexivity. cbn.
+      econstructor. }
+    { eexists. eapply rtc_once. exists [].
+      eapply step_atomic with (t1:=[]). 1,2: reflexivity. cbn.
+      eapply ectx_language.Ectx_step with (K:=[]). 1,2: reflexivity. cbn.
+      econstructor. }
+    { apply IHfuel in Hc as [φ' Hc]. eexists.
+      eapply rtc_l. exists [].
+      eapply step_atomic with (t1:=[]). 1,2: reflexivity. cbn.
+      eapply ectx_language.Ectx_step with (K:=[]). 1,2: reflexivity. cbn.
+      econstructor. cbn. apply Hc. } }
+Qed.
+
